oracle_comp_pair type for access to multiple oracles

src/crypto_foundations/primitives/hash_function/hash_function.lean
@@ -10,107 +10,120 @@ This file defines the notion of a keyed hash function.
 TODO: Think about using `encodable` type-class
 -/
 
-section hash_f
+def negligable_expirement_success (exp : ℕ → comp bool) (h : ∀ sp, (exp sp).is_well_formed) : Prop :=
+asymptotics.negligable (λ sp, comp.Pr (exp sp))
 
-structure hash_f (K I O : Type) :=
+structure hash_function (K I O : Type) :=
 (keygen : comp K)
 (keygen_is_well_formed : keygen.is_well_formed)
 (hash (key : K) (m : I) : O)
 
-variables {K I O : Type} (h : hash_f K I O)
+namespace hash_function
+
+variables {K I O : Type} (h : hash_function K I O)
 
 @[simp]
-instance hash_f.keygen.is_well_formed (h : hash_f K I O) :
+instance keygen.is_well_formed (h : hash_function K I O) :
   h.keygen.is_well_formed :=
 h.keygen_is_well_formed
 
 variables [decidable_eq O]
 
 /-- The security game for collision resistance as a probabalistic function. -/
-def hash_f.collision_finding_experiment (h : hash_f K I O) 
-  (a : K → comp (I × I)) : comp bool :=
+def collision_finding_experiment (h : hash_function K I O) 
+  (A : K → comp (I × I)) : comp bool :=
 comp.bind (h.keygen) (λ k,
-comp.bind (a k) (λ xs, 
+comp.bind (A k) (λ xs, 
 comp.ret (h.hash k xs.1 = h.hash k xs.2)))
 
 @[simp]
-lemma collision_finding_experiment_is_well_formed_iff (h : hash_f K I O)
+lemma collision_finding_experiment_is_well_formed_iff (h : hash_function K I O)
   (a : K → comp (I × I)) : 
   (h.collision_finding_experiment a).is_well_formed ↔ 
     (∀ (k : K), k ∈ (h.keygen).support → (a k).is_well_formed)  :=
-by simp [hash_f.collision_finding_experiment]
+by simp [collision_finding_experiment]
 
-instance collision_finding_experiment.is_well_formed (h : hash_f K I O) 
-  (a : K → comp (I × I)) [ha : ∀ k, (a k).is_well_formed] :
+instance collision_finding_experiment.is_well_formed (h : hash_function K I O) 
+  (a : K → comp (I × I)) (ha : ∀ k, (a k).is_well_formed) :
   (h.collision_finding_experiment a).is_well_formed :=
 begin
   rw [collision_finding_experiment_is_well_formed_iff],
   exact λ k _, ha k,
 end
 
-end hash_f
-
-section hash_scheme
+end hash_function
 
 /-- `keygen` takes in a security parameter and outputs a key bundled with the parameter
   `hash` takes a `hash_key` from keygen and a string in the input space to a string in the output space -/
 structure hash_scheme (K I O : ℕ → Type) :=
-(scheme (sp : ℕ) : hash_f (K sp) (I sp) (O sp))
+(scheme (sp : ℕ) : hash_function (K sp) (I sp) (O sp))
 (keygen_poly_time : complexity_class.poly_time_comp₀ (λ sp, (scheme sp).keygen))
 (hash_poly_time : complexity_class.poly_time_fun₂ (λ sp, (scheme sp).hash))
 
-variables {K I O : ℕ → Type} (H : hash_scheme K I O)
+namespace hash_scheme
+
+variables {K I O : ℕ → Type} {H : hash_scheme K I O}
 
 section projections
 
-def hash_scheme.keygen (sp : ℕ) : comp (K sp) :=
+variable (H)
+
+def keygen (sp : ℕ) : comp (K sp) :=
 (H.scheme sp).keygen
 
 @[simp]
-lemma hash_scheme.keygen_eq (sp : ℕ) :
+lemma keygen_eq (sp : ℕ) :
   H.keygen sp = (H.scheme sp).keygen := rfl
 
-def hash_scheme.hash {sp : ℕ} (k : K sp) (i : I sp) : O sp :=
+def hash {sp : ℕ} (k : K sp) (i : I sp) : O sp :=
 (H.scheme sp).hash k i
 
 @[simp]
-lemma hash_scheme.hash_eq {sp : ℕ} (k : K sp) (i : I sp) :
+lemma hash_eq {sp : ℕ} (k : K sp) (i : I sp) :
   H.hash k i = (H.scheme sp).hash  k i:= rfl
 
 end projections
 
 variables [∀ n, decidable_eq $ O n]
 
+def collision_finding_adversary (H : hash_scheme K I O) :=
+Π (sp : ℕ), K sp → comp ((I sp) × (I sp))
+
+class collision_finding_adversary.admissable {H : hash_scheme K I O}
+  (A : collision_finding_adversary H) :=
+(is_well_formed : ∀ sp k, (A sp k).is_well_formed)
+(poly_time : complexity_class.poly_time_comp₁ A)
+
+instance collision_finding_adversary.is_well_formed
+  {H : hash_scheme K I O} {A : collision_finding_adversary H}
+  (hA : A.admissable) (sp : ℕ) (k : K sp) :
+  (A sp k).is_well_formed :=
+collision_finding_adversary.admissable.is_well_formed H sp k
+
 /-- The security game for collision resistance as a probabalistic function. 
   Adversary implicitly recieves the secuirty parameter via the hashkey from `keygen`-/
-def hash_scheme.collision_finding_experiment (H : hash_scheme K I O) 
-  (A : Π (sp : ℕ), K sp → comp ((I sp) × (I sp))) (sp : ℕ) : comp bool :=
+def collision_finding_experiment (H : hash_scheme K I O) 
+  (A : collision_finding_adversary H) (sp : ℕ) : comp bool :=
 (H.scheme sp).collision_finding_experiment (A sp)
 
 @[simp]
-lemma hash_scheme.collision_finding_experiment_is_well_formed_iff
-  (H : hash_scheme K I O) (A : Π (sp : ℕ), K sp → comp ((I sp) × (I sp))) (sp : ℕ) :
+lemma collision_finding_experiment_is_well_formed_iff (H : hash_scheme K I O) 
+  (A : collision_finding_adversary H) (sp : ℕ) :
   (H.collision_finding_experiment A sp).is_well_formed ↔
     ∀ k ∈ (H.keygen sp).support, (A sp k).is_well_formed :=
 by simp [hash_scheme.collision_finding_experiment]
 
-instance hash_scheme.collision_finding_experiment.is_well_formed (H : hash_scheme K I O)
-  (A : Π (sp : ℕ), K sp → comp ((I sp) × (I sp))) (sp : ℕ)
-  [hA : ∀ k, (A sp k).is_well_formed] :
+instance collision_finding_experiment.is_well_formed (H : hash_scheme K I O)
+  (A : collision_finding_adversary H) (hA : A.admissable) (sp : ℕ) :
   (H.collision_finding_experiment A sp).is_well_formed :=
 begin
-  rw hash_scheme.collision_finding_experiment_is_well_formed_iff,
-  exact λ k hk, hA k,
+  refine hash_function.collision_finding_experiment.is_well_formed _ _ _,
+  refine collision_finding_adversary.is_well_formed hA sp,
 end
 
-def negligable_expirement_success (exp : ℕ → comp bool) (h : ∀ sp, (exp sp).is_well_formed) : Prop :=
-asymptotics.negligable (λ sp, comp.Pr (exp sp))
-
--- TODO: make an admissable adversary
 def collision_resistant (H : hash_scheme K I O) : Prop :=
-∀ (A : Π (sp : ℕ), K sp → comp ((I sp) × (I sp)))
-  (A_efficient : complexity_class.poly_time_comp₁ A)
-  [A_well_formed : ∀ (sp : ℕ) (k : K sp) (hk : k ∈ (H.keygen sp).support), (A sp k).is_well_formed],
-negligable_expirement_success (H.collision_finding_experiment A) (by simpa)
+∀ (A : collision_finding_adversary H) (hA : A.admissable),
+negligable_expirement_success (H.collision_finding_experiment A)
+  (collision_finding_experiment.is_well_formed H A hA)
 
 end hash_scheme
