src/crypto_foundations/oracle_comp_pair.lean
@@ -1,0 +1,38 @@
+import crypto_foundations.oracle_comp
+
+open oracle_comp
+
+def oracle_comp_pair (A B A' B' C : Type) :=
+oracle_comp (A ⊕ A') (B ⊕ B') C
+
+@[simps]
+instance oracle_comp_pair.monad {A B A' B' : Type} :
+  monad (oracle_comp_pair A B A' B') :=
+{ pure := λ C c, oc_ret (comp.ret c),
+  bind := λ A B ca cb, oc_bind ca cb }
+
+namespace oracle_comp_pair
+
+variables {A B A' B' C : Type}
+
+def eval_distribution {S S' : Type}
+  (oc : oracle_comp_pair A B A' B' C)
+  (s : S) (o : S → A → comp (B × S))
+  (s' : S') (o' : S' → A' → comp (B' × S')) :
+  comp (C × (S × S')) :=
+begin
+  refine oc.eval_distribution (s, s') (λ ss' aa', _),
+  refine aa'.rec (λ a, _) (λ a', _),
+  refine (o ss'.1 a) >>= (λ bs, comp.ret ⟨(sum.inl bs.1), (bs.2, ss'.2)⟩),
+  refine (o' ss'.2 a') >>= (λ bs', comp.ret ⟨(sum.inr bs'.1), (ss'.1, bs'.2)⟩),
+end
+
+def query_left (a : A) : oracle_comp_pair A B A' B' (with_bot B) :=
+do bb' ← (oc_query (sum.inl a)), 
+  return (bb'.rec (λ b, ↑b) (λ _, ⊥))
+
+def query_right (a' : A') : oracle_comp_pair A B A' B' (with_bot B') :=
+do bb' ← (oc_query (sum.inr a')),
+  return (bb'.rec (λ _, ⊥) (λ b', ↑b'))
+
+end oracle_comp_pair
